\documentclass{zc-ust-hw}

\usepackage{lipsum}

\newcommand*{\name}{SalahDin Rezk}
\newcommand*{\id}{202201079}
\newcommand*{\course}{Linear Algebra and Vector Geometry (MATH 201)}
\newcommand*{\assignment}{Bonus 1}

\begin{document}

\maketitle

Prove that $(AB)^\intercal=B^\intercal A^\intercal$ \\

\begin{proof}
  Let $A$ be an $m\times n$ matrix and $B$ be an $n\times p$ matrix.

  \begin{align}
    A_{ij} &= \sum_{i=1}^m \sum_{j=1}^n a_{ij} \\
    B_{ij} &= \sum_{i=1}^n \sum_{j=1}^p b_{ij}
  .\end{align}
  Using the definition of matrix multiplication:
  \begin{align}
    AB_{ij} &= \sum_{k=1}^n a_{ik}b_{kj}
  .\end{align}
  Using definition of transpose:
  \begin{align}
    (AB)^\intercal_{ij} &= AB_{ji} \\
                        &= \sum_{k=1}^n a_{jk}b_{ki} \label{eq:1}
  .\end{align}
  Then:
  \begin{align}
    (B^\intercal A^\intercal)_{ij} &= \sum_{k=1}^n b_{ik}^\intercal a_{kj}^\intercal \\
                                   &= \sum_{k=1}^n b_{ki}a_{jk} \\
                                   &= \sum_{k=1}^n a_{jk}b_{ki} \label{eq:2}
  .\end{align}
  From \eqref{eq:1} and \eqref{eq:2} we conclude that $(AB)^\intercal=B^\intercal A^\intercal$.
\end{proof}
\vspace{1em}
Notice that $(AB)^\intercal\neq A^\intercal B^\intercal$.

\end{document}
